proof/invariants/findBlockInKSWithAddr.v
@@ -36,11 +36,12 @@
 Require Import Model.Monad Model.Lib Model.MAL.
 Require Import Core.Internal.
 Require Import Proof.Consistency Proof.DependentTypeLemmas Proof.Hoare
-               Proof.Isolation Proof.StateLib Proof.WeakestPreconditions Proof.invariants.Invariants.
-Require Import Compare_dec Bool List.
+               Proof.Isolation Proof.StateLib Proof.WeakestPreconditions
+			   Proof.invariants.Invariants Proof.InternalLemmas.
+Require Import Compare_dec Bool List Coq.Logic.ProofIrrelevance Lia.
 
 Lemma findBlockInKSWithAddrAux n (kernelstructurestart blockEntryAddr : paddr) (P : state -> Prop) :
-{{  fun s : state => P s /\ consistency s
+{{  fun (s : state)  => P s /\ consistency s
 										/\ isKS kernelstructurestart s}}
 Internal.findBlockInKSWithAddrAux n kernelstructurestart blockEntryAddr
 {{fun (blockaddr : paddr) (s : state) => P s /\ consistency s /\
@@ -48,13 +49,14 @@ Internal.findBlockInKSWithAddrAux n kernelstructurestart blockEntryAddr
 																	(exists entry, lookup blockaddr s.(memory) beqAddr = Some (BE entry)
 																			/\ blockaddr = blockEntryAddr
 																			/\ bentryPFlag blockaddr true s
-																			(*/\ In blockaddr (filterOptionPaddr((getKSEntriesAux n
+																			/\ In blockaddr (filterOptionPaddr(getKSEntriesAux n
 																																kernelstructurestart
-																																s (CIndex maxNbPrepare))))*)
-)) }}.
+																																s ))
+																																)
+) }}.
 Proof.
 (* revert mandatory to generalize the induction hypothesis *)
-revert kernelstructurestart blockEntryAddr.
+revert kernelstructurestart blockEntryAddr P.
 	induction n.
 - (* n = 0 *)
 	intros;simpl.
@@ -82,8 +84,8 @@ revert kernelstructurestart blockEntryAddr.
 	}
 	intro maxEntryAddrInStructure.
 	eapply bindRev.
-	{ (** leb *)
-		eapply weaken. apply Paddr.leb.
+	{ (** ltb *)
+		eapply weaken. apply Paddr.ltb.
 		intros. simpl. apply H.
 	}
 	intro isEntryAddrBelowEnd.
@@ -106,16 +108,277 @@ revert kernelstructurestart blockEntryAddr.
 					}
 					intro isPresent.
 					case_eq isPresent.
-						-- (* case_eq isPresent = true *)
-							intros. simpl. eapply weaken. apply ret.
-							intros. simpl. intuition.
-							right. apply isBELookupEq in H10. destruct H10. exists x. intuition.
-						-- (* case_eq isPresent = false *)
-							intros. eapply weaken. apply ret.
-							intros. simpl. intuition.
-				* (* case_eq entryExists = false *)
-					intros. simpl. eapply weaken. apply ret.
+					-- (* case_eq isPresent = true *)
+						intros. simpl. eapply weaken. apply ret.
+						intros. simpl. intuition.
+						assert(HBE : isBE blockEntryAddr s)
+							by intuition.
+						right. apply isBELookupEq in HBE. destruct HBE.
+						exists x. intuition.
+
+						assert(HNextKSOffsetIsPADDR : NextKSOffsetIsPADDR s)
+							by (unfold consistency in * ; unfold consistency1 in * ; intuition).
+						unfold NextKSOffsetIsPADDR in *.
+						assert(HisKScurr : isKS kernelstructurestart s) by intuition.
+						specialize (HNextKSOffsetIsPADDR kernelstructurestart
+														(CPaddr (kernelstructurestart + nextoffset))
+														HisKScurr).
+						assert(HNextKSIsKS : NextKSIsKS s)
+								by (unfold consistency in * ; unfold consistency1 in * ; intuition).
+						unfold NextKSIsKS in *.
+						specialize (HNextKSIsKS kernelstructurestart
+															(CPaddr (kernelstructurestart + nextoffset))).
+						unfold nextKSAddr in *.
+						unfold isKS in *.
+						destruct (lookup kernelstructurestart (memory s) beqAddr) eqn:Hlookupcurr ; try(exfalso ; congruence).
+						destruct v ; try(exfalso ; congruence).
+						unfold isPADDR in *.
+						intuition.
+						unfold nextKSentry in *. subst.
+
+						unfold Paddr.addPaddrIdx.
+						unfold CPaddr in *.
+						simpl in *.
+						
+						destruct (le_dec (kernelstructurestart + nextoffset) maxAddr) eqn:Hnextoffset ; try lia.
+						---	(* nextaddr is well formed *)
+							assert(HpEq : ADT.CPaddr_obligation_1 (kernelstructurestart + nextoffset) l =
+													StateLib.Paddr.addPaddrIdx_obligation_1 kernelstructurestart
+										nextoffset l).
+							{ apply proof_irrelevance. }
+							rewrite HpEq in *.
+
+							destruct (lookup
+											{|
+											p := kernelstructurestart + nextoffset;
+											Hp :=
+												StateLib.Paddr.addPaddrIdx_obligation_1 kernelstructurestart
+												nextoffset l
+											|} (memory s) beqAddr) eqn:Hlookupnext ; intuition.
+													destruct v ; intuition.
+
+							specialize (HNextKSIsKS	p HisKScurr).
+							intuition.
+
+							destruct (beqAddr p nullAddr) eqn:beqpNull.
+							---- (* p = nullAddr *)
+									(* there is no following struct *)
+									rewrite <- DependentTypeLemmas.beqAddrTrue in beqpNull.
+									rewrite beqpNull in *.
+
+									assert(HnullAddrExists : nullAddrExists s)
+										by (unfold consistency in * ; unfold consistency1 in * ; intuition).
+									unfold nullAddrExists in *. unfold isPADDR in *.
+
+									destruct (lookup nullAddr (memory s) beqAddr) eqn:Hlookupp ; intuition ; try(exfalso ; congruence).
+									destruct v ; intuition ; try(exfalso ; congruence).
+
+									assert(HidxEq : CIndex 7 = CIndex (kernelStructureEntriesNb-1)).
+									{
+										unfold CIndex. simpl in *.
+										destruct (le_dec 7 maxIdx) ; trivial.
+									}
+
+									assert(kernelStructureEntriesNb < maxIdx-1)
+										by (apply KSEntriesNbLessThanMaxIdx).
+
+									assert(kernelStructureEntriesNb-1 < maxIdx)
+										by lia.
+
+									assert(CIndex (kernelStructureEntriesNb-1) < CIndex kernelStructureEntriesNb).
+									{
+										unfold CIndex.
+										destruct (le_dec (kernelStructureEntriesNb - 1) maxIdx) ; intuition.
+										destruct (le_dec kernelStructureEntriesNb maxIdx) ; intuition.
+									}
+									assert((CIndex (kernelStructureEntriesNb - 1) < maxIdx+1)).
+									{
+										unfold CIndex. 
+										destruct (le_dec (kernelStructureEntriesNb - 1) maxIdx) ; intuition.
+									}
+									assert(CIndex (kernelStructureEntriesNb - 1) < kernelStructureEntriesNb).
+									{
+										unfold CIndex. 
+										destruct (le_dec (kernelStructureEntriesNb - 1) maxIdx) ; intuition.
+									}
+									rewrite andb_true_iff in H.
+
+									eapply blockInRangeInStruct ; intuition ; try lia.
+									intuition.
+									
+									unfold sh1offset in *. unfold blkoffset in *.
+									simpl in *.
+									rewrite PeanoNat.Nat.add_0_r in *.
+
+									assert(beqAddr blockEntryAddr nullAddr = false).
+									{
+										rewrite <- beqAddrFalse. intro Hfalse.
+										rewrite Hfalse in *.
+										unfold isBE in *.
+										rewrite Hlookupp in *.
+										exfalso ; congruence.
+									}
+
+									assert(kernelStructureEntriesNb-1 < sh1offset).
+									{
+										unfold sh1offset. unfold blkoffset.
+										unfold CIndex.
+										destruct (le_dec 0 maxIdx) ; intuition ; simpl.
+										destruct (le_dec kernelStructureEntriesNb maxIdx) ; intuition.
+									}
+
+									assert(HwellFormedSh1 : wellFormedFstShadowIfBlockEntry s)
+										by (unfold consistency in * ; unfold consistency1 in * ; intuition).
+									unfold wellFormedFstShadowIfBlockEntry.
+									assert(HBE : isBE kernelstructurestart s)
+										by (unfold isBE ; rewrite Hlookupcurr ; trivial).
+									specialize (HwellFormedSh1 kernelstructurestart HBE).
+									unfold isSHE in *.
+
+									unfold StateLib.Paddr.leb in *.
+									simpl in *.
+									rewrite PeanoNat.Nat.leb_le in *.
+									unfold StateLib.Paddr.ltb in *.
+									rewrite PeanoNat.Nat.ltb_lt in *.
+									rewrite PeanoNat.Nat.le_neq in *.
+									intuition.
+
+									destruct (le_dec (kernelstructurestart + CIndex kernelStructureEntriesNb) maxAddr) ; intuition.
+
+									unfold CPaddr in *.
+									destruct (le_dec (kernelstructurestart + sh1offset) maxAddr) ; intuition.
+									unfold CIndex in *. simpl in *.
+									destruct (le_dec 7 maxIdx) ; intuition. simpl in *.
+									assert(HEqpred : 7 = kernelStructureEntriesNb-1) by intuition.
+									rewrite HEqpred in *.
+									destruct (le_dec (kernelstructurestart + (kernelStructureEntriesNb - 1)) maxAddr) ; intuition ; try lia.
+									destruct (le_dec kernelStructureEntriesNb maxIdx) ; intuition ; try lia.
+									destruct blockEntryAddr. simpl in *.
+									assert(HEqpred' :7 = kernelStructureEntriesNb-1) by intuition.
+									rewrite HEqpred' in *.
+									lia.
+
+									unfold isKS.
+									rewrite Hlookupcurr. intuition.
+
+									(*unfold isBE. rewrite H5. trivial.*)
+
+							---- (* p <> nullAddr *)
+								(* DUP *)
+								rewrite <- beqAddrFalse in beqpNull.
+								intuition.
+								destruct (lookup p (memory s) beqAddr) eqn:Hlookupp ; intuition.
+								destruct v ; intuition.
+
+								unfold StateLib.Index.pred.
+
+								(*assert(maxNbPrepare < maxIdx - 1)
+									by apply maxNbPrepareNbLessThanMaxIdx.
+
+								destruct (le_dec maxNbPrepare maxIdx) ; intuition ; try lia.
+								simpl.*)
+
+								rewrite filterOptionPaddrSplit.
+								rewrite in_app_iff. left.
+
+								assert(HEqpred : 7 = kernelStructureEntriesNb-1) by intuition.
+								rewrite HEqpred in *.
+
+								assert(kernelStructureEntriesNb < maxIdx-1)
+									by (apply KSEntriesNbLessThanMaxIdx).
+
+								assert(kernelStructureEntriesNb-1 < maxIdx)
+									by lia.
+
+								unfold CIndex.
+								destruct (le_dec (kernelStructureEntriesNb - 1) maxIdx) ; intuition ; try lia.
+
+								rewrite andb_true_iff in H.
+								eapply blockInRangeInStruct ; intuition ; try lia.
+
+								unfold sh1offset in *. unfold blkoffset in *.
+								simpl in *.
+								rewrite PeanoNat.Nat.add_0_r in *.
+
+								assert(beqAddr blockEntryAddr nullAddr = false).
+								{
+									rewrite <- beqAddrFalse. intro Hfalse.
+									rewrite Hfalse in *.
+									unfold isBE in *.
+									assert(HnullAddrExists : nullAddrExists s)
+										by (unfold consistency in * ; unfold consistency1 in * ; intuition).
+									unfold nullAddrExists in *. unfold isPADDR in *.
+
+									destruct (lookup nullAddr (memory s) beqAddr) eqn:Hlookupnull ; intuition ; try(exfalso ; congruence).
+									destruct v ; intuition ; try(exfalso ; congruence).
+								}
+
+								unfold CIndex in *.
+								destruct (le_dec kernelStructureEntriesNb maxIdx) ; intuition.
+								simpl in *.
+
+								assert(kernelStructureEntriesNb-1 < sh1offset).
+								{
+									unfold sh1offset. unfold blkoffset.
+									unfold CIndex.
+									destruct (le_dec 0 maxIdx) ; intuition ; simpl.
+									destruct (le_dec kernelStructureEntriesNb maxIdx) ; intuition.
+								}
+
+								assert(HwellFormedSh1 : wellFormedFstShadowIfBlockEntry s)
+									by (unfold consistency in * ; unfold consistency1 in * ; intuition).
+								unfold wellFormedFstShadowIfBlockEntry.
+								assert(HBE : isBE kernelstructurestart s)
+									by (unfold isBE ; rewrite Hlookupcurr ; trivial).
+								specialize (HwellFormedSh1 kernelstructurestart HBE).
+								unfold isSHE in *.
+
+								destruct (le_dec (kernelstructurestart + kernelStructureEntriesNb) maxAddr) ; intuition.
+								
+								unfold StateLib.Paddr.leb in *.
+								simpl in *.
+								rewrite PeanoNat.Nat.leb_le in *.
+								unfold StateLib.Paddr.ltb in *.
+								rewrite PeanoNat.Nat.ltb_lt in *.
+								rewrite PeanoNat.Nat.le_neq in *.
+								intuition.
+
+								unfold CPaddr. unfold CIndex. simpl in *.
+								(*destruct (le_dec 7 maxIdx) ; intuition. simpl in *.*)
+								assert(HEqpred' : 7 = kernelStructureEntriesNb-1) by intuition.
+								rewrite HEqpred' in *.
+								destruct (le_dec (kernelstructurestart + (kernelStructureEntriesNb - 1)) maxAddr) ; intuition ; try lia.
+								destruct blockEntryAddr. simpl in *.
+								assert(HEqpred'': 7 = kernelStructureEntriesNb-1) by intuition.
+								rewrite HEqpred'' in *.
+								lia.
+
+								unfold isKS.
+								rewrite Hlookupcurr. intuition.
+										
+						--- (* next is not well formed, contradiction *)
+							intuition.
+						
+							assert(HnullAddrExists : nullAddrExists s)
+								by (unfold consistency in * ; unfold consistency1 in * ; intuition).
+							unfold nullAddrExists in *. unfold isPADDR in *.
+
+							destruct (lookup nullAddr (memory s) beqAddr) eqn:Hlookupp ; intuition ; try(exfalso ; congruence).
+							destruct v ; intuition ; try(exfalso ; congruence).
+
+							unfold nullAddr in *.
+							unfold CPaddr in *.
+							destruct (le_dec 0 maxAddr) ; intuition.
+							assert(HpEq : ADT.CPaddr_obligation_1 0 l = ADT.CPaddr_obligation_2)
+								by apply proof_irrelevance.
+							rewrite HpEq in *.
+							exfalso ; congruence.
+				-- (* case_eq isPresent = false *)
+					intros. eapply weaken. apply ret.
 					intros. simpl. intuition.
+			* (* case_eq entryExists = false *)
+				intros. simpl. eapply weaken. apply ret.
+				intros. simpl. intuition.
 		+	(* case_eq isEntryAddrAboveStart && isEntryAddrBelowEnd = false *)
 			intros.
 			eapply bindRev.
@@ -140,36 +403,127 @@ revert kernelstructurestart blockEntryAddr.
 					}
 				* (* case_eq isnull = false *)
 					{ (** induction hypothesis *)
-						intros. eapply weaken. apply IHn.
-						intros. simpl. intuition.
-						apply isKSLookupEq in H10. destruct H10 as [x (H10&Hblockidx)].
-						destruct H4. intuition.
-						assert(HnextKSIsKS : NextKSIsKS s)
-							by (unfold consistency in * ; unfold consistency1 in * ; intuition).
-						unfold NextKSIsKS in *.
-						apply HnextKSIsKS with 	(addr:=kernelstructurestart)
-																		(nextKSaddr:=CPaddr (kernelstructurestart + nextoffset))
-																		(nextKS:=nextKernelStructure) ;
-						intuition.
-						- unfold isKS. rewrite H10 ; trivial.
-						- unfold nextKSAddr. rewrite H10 ; trivial.
-						- unfold nextKSentry in *. subst x0. intuition.
-						(* Prove nextKernelStructure <> nullAddr *)
-						- apply beqAddrFalse in H3. intuition.
+						intros.
+						eapply strengthen. eapply weaken.
+						
+						+	eapply IHn.
+						+	intros. simpl. split. apply H1. intuition.
+							assert(HKS : isKS kernelstructurestart s)
+								by intuition.
+							apply isKSLookupEq in HKS. destruct HKS as [x (HKS&Hblockidx)].
+							destruct H4. (*exists offset : paddr,
+												(offset = ...*)
+							intuition.
+							assert(HnextKSIsKS : NextKSIsKS s)
+								by (unfold consistency in * ; unfold consistency1 in * ; intuition).
+							unfold NextKSIsKS in *.
+							apply HnextKSIsKS with 	(addr:=kernelstructurestart)
+													(nextKSaddr:=CPaddr (kernelstructurestart + nextoffset))
+													(nextKS:=nextKernelStructure) ;
+							intuition.
+							- unfold nextKSAddr. rewrite HKS ; trivial.
+							- unfold nextKSentry in *. subst x0. intuition.
+							(* Prove nextKernelStructure <> nullAddr *)
+							- rewrite <- beqAddrFalse in *. intuition.
+						+ intros. simpl in *. intuition.
+							(* block in next ks *)
+							right.
+							destruct H11. (*  exists entry : BlockEntry, ...*)
+							intuition.
+							exists x. intuition.
+							subst.
+							destruct H6 as [offset Hoffset]. (* exists offset : paddr,
+																(offset = ...*)
+							destruct Hoffset as [Hoffset HnextKSentry].
+							destruct Hoffset as [Hoffset HnextKSaddr].
+							assert(HNextKSOffsetIsPADDR : NextKSOffsetIsPADDR s)
+								by (unfold consistency in * ; unfold consistency1 in * ; intuition).
+							unfold NextKSOffsetIsPADDR in *.
+							assert(HisKScurr : isKS kernelstructurestart s) by intuition.
+							specialize (HNextKSOffsetIsPADDR kernelstructurestart
+															(CPaddr (kernelstructurestart + nextoffset))
+															HisKScurr).
+							assert(HNextKSIsKS : NextKSIsKS s)
+									by (unfold consistency in * ; unfold consistency1 in * ; intuition).
+							unfold NextKSIsKS in *.
+							specialize (HNextKSIsKS kernelstructurestart
+																(CPaddr (kernelstructurestart + nextoffset))).
+							unfold nextKSAddr in *.
+							unfold isKS in *.
+							destruct (lookup kernelstructurestart (memory s) beqAddr) eqn:Hlookupcurr ; try(exfalso ; congruence).
+							destruct v ; try(exfalso ; congruence).
+							unfold isPADDR in *.
+							intuition.
+							unfold nextKSentry in *. subst.
+
+							unfold Paddr.addPaddrIdx.
+							unfold CPaddr in *.
+							simpl in *.
+							
+							destruct (le_dec (kernelstructurestart + nextoffset) maxAddr) eqn:Hnextoffset ; try lia.
+							---	(* nextaddr is well formed *)
+								assert(HpEq : ADT.CPaddr_obligation_1 (kernelstructurestart + nextoffset) l =
+														StateLib.Paddr.addPaddrIdx_obligation_1 kernelstructurestart
+											nextoffset l).
+								{ apply proof_irrelevance. }
+								rewrite HpEq in *.
+
+								destruct (lookup
+												{|
+												p := kernelstructurestart + nextoffset;
+												Hp :=
+													StateLib.Paddr.addPaddrIdx_obligation_1 kernelstructurestart
+													nextoffset l
+												|} (memory s) beqAddr) eqn:Hlookupnext ; intuition.
+														destruct v ; intuition.
+
+								specialize (HNextKSIsKS	p HisKScurr).
+								intuition.
+								subst.
+
+								destruct (beqAddr p nullAddr) eqn:beqpNull.
+								---- (* p = nullAddr *)
+										(* there is no following struct *)
+										rewrite <- DependentTypeLemmas.beqAddrTrue in beqpNull.
+										rewrite beqpNull in *.
+
+										assert(HnullAddrExists : nullAddrExists s)
+											by (unfold consistency in * ; unfold consistency1 in * ; intuition).
+										unfold nullAddrExists in *. unfold isPADDR in *.
+
+										destruct (lookup nullAddr (memory s) beqAddr) eqn:Hlookupp ; intuition ; try(exfalso ; congruence).
+								---- (* p <> nullAddr *)
+										rewrite <- beqAddrFalse in beqpNull.
+										intuition.
+
+										destruct (lookup p (memory s) beqAddr) eqn:Hlookupp ; intuition.
+										destruct v ; intuition.
+
+										rewrite filterOptionPaddrSplit.
+										rewrite in_app_iff. right.
+										intuition.
+							--- (* false, nulladdr not null *)
+								unfold nullAddr in *.
+								unfold CPaddr in *.
+								destruct (le_dec 0 maxAddr) ; intuition.
+								assert(HpEq : ADT.CPaddr_obligation_2 =
+										ADT.CPaddr_obligation_1 0 l)
+									by apply proof_irrelevance.
+								rewrite HpEq in *.
+								congruence.
 					}
 Qed.
-
 
 
 Lemma findBlockInKSWithAddr (idPD blockEntryAddr: paddr) (P : state -> Prop) :
 {{ fun s => P s /\ consistency s /\ isPDT idPD s}}
 Internal.findBlockInKSWithAddr idPD blockEntryAddr 
 {{fun (blockaddr : paddr) (s : state) => P s /\ consistency s /\
-																				(blockaddr = nullAddr \/
-																	(exists entry, lookup blockaddr s.(memory) beqAddr = Some (BE entry)
-																			/\ blockaddr = blockEntryAddr
-																			/\ bentryPFlag blockaddr true s
-																			/\ In blockaddr (getMappedBlocks idPD s))) }}.
+										(blockaddr = nullAddr \/
+											(exists entry, lookup blockaddr s.(memory) beqAddr = Some (BE entry)
+													/\ blockaddr = blockEntryAddr
+													/\ bentryPFlag blockaddr true s
+													/\ In blockaddr (getMappedBlocks idPD s))) }}.
 Proof.
 unfold Internal.findBlockInKSWithAddr.
 eapply bindRev.
@@ -177,32 +531,75 @@ eapply bindRev.
 	eapply weaken. apply readPDStructurePointer.
 	intros. simpl. split. apply H. intuition.
 }
-	intro kernelstructurestart.
-	(** findBlockInKSWithAddrAux *)
+intro kernelstructurestart.
+eapply bindRev.
+{ (** Internal.compareAddrToNull *)
+	eapply weaken. apply compareAddrToNull.
+	intros. simpl. apply H.
+}
+intro kernelstructureisnull.
+case_eq kernelstructureisnull.
++ (* case_eq kernelstructureisnull = true *)
+	intros.
+	{ (** ret *)
+		eapply weaken. apply ret.
+		intros. simpl. intuition.
+	}
++ (* case_eq kernelstructureisnull = false *)
+	intro Hkernelstructureisnull. simpl.
+	{ (** findBlockInKSWithAddrAux *)
 	eapply strengthen. eapply weaken. apply findBlockInKSWithAddrAux ; intuition.
 	intros. simpl in *. split. apply H. intuition.
-	assert(HSPIsKS : StructurePointerIsKS s)
+	rewrite <- beqAddrFalse in *. intuition.
+	assert(HPDT : isPDT idPD s)
+		by assumption.
+	apply isPDTLookupEq in HPDT. destruct HPDT as [pdentry Hlookuppd].
+
+	assert(HStructurePointerIsKS : StructurePointerIsKS s)
 		by (unfold consistency in * ; unfold consistency1 in * ; intuition).
-	unfold isPDT in *.
-	destruct (lookup idPD (memory s) beqAddr) eqn:Hlookup ; try (exfalso; congruence).
-	destruct v eqn:Hv ; try (exfalso; congruence).
+	unfold StructurePointerIsKS in *.
+	specialize (HStructurePointerIsKS idPD pdentry Hlookuppd).
 	unfold pdentryStructurePointer in *.
-	rewrite Hlookup in H1.
-	subst.
-	apply HSPIsKS with idPD.
-	assumption.
-	intros. simpl in *. intuition.
-	(*right. destruct H4 as [bentry Hbentry]. exists bentry. intuition.
+	rewrite Hlookuppd in *. subst. intuition.
+	
+	intros. intuition. apply H. apply H. intuition.
+	(* block in next ks *)
+	right.
+	rewrite <- beqAddrFalse in *.
+	intuition.
+	destruct H5 as [bentry Hbentry]. (* exists entry : BlockEntry,
+										lookup a (memory s) beqAddr = Some (BE entry)... *)
+	exists bentry. intuition.
 	subst a.
+	
 	unfold getMappedBlocks. unfold getKSEntries.
-	apply isPDTLookupEq in H5. destruct H5 as [pdentry Hlookuppdentry].
+	assert(HPDT : isPDT idPD s)
+		by intuition.
+	apply isPDTLookupEq in HPDT. destruct HPDT as [pdentry Hlookuppdentry].
 	unfold pdentryStructurePointer in *. rewrite Hlookuppdentry in *.
 	subst kernelstructurestart.
-	destruct (beqAddr (structure pdentry) nullAddr).
-	admit.
-	induction (maxIdx+1).
-	- simpl in *. intuition.*)
-Admitted.
+	destruct (beqAddr (structure pdentry) nullAddr) eqn:HstructureNull.
+	- (* (structure pdentry) = nullAddr *)
+		rewrite <- DependentTypeLemmas.beqAddrTrue in HstructureNull.
+		exfalso ; congruence.
+	-  (* (structure pdentry) <> nullAddr *)
+		unfold N in *. assert(HmaxEq :  maxIdx = maxAddr) by apply maxIdxEqualMaxAddr.
+		rewrite HmaxEq in *.
+
+		induction ((filterOptionPaddr (getKSEntriesAux (maxAddr + 1) (structure pdentry) s (*(CIndex maxNbPrepare)*)))).
+		-- intuition.
+		-- simpl in *. intuition.
+			--- (* a = blockEntryAddr *)
+				subst blockEntryAddr.
+				rewrite H4. (* lookup a ... *)
+				unfold bentryPFlag in *. rewrite H4 in *.
+				rewrite <- H5 in *. (* true = present bentry *)
+				intuition.
+			--- destruct (lookup a (memory s) beqAddr) ; intuition.
+				destruct v ; intuition.
+				destruct (present b) ; intuition.
+	}
+Qed.
 
 
 
